compiler/backend/backendScript.sml
@@ -260,7 +260,7 @@ val to_livesets_def = Define`
   to_livesets (c:α backend$config) p =
   let (c',p) = to_data c p in
   let (data_conf,word_conf,asm_conf) = (c.data_conf,c.word_to_word_conf,c.lab_conf.asm_conf) in
-  let p = stubs(:α) ++ MAP (compile_part data_conf) p in
+  let p = stubs(:α) data_conf ++ MAP (compile_part data_conf) p in
   let (two_reg_arith,reg_count) = (asm_conf.two_reg_arith, asm_conf.reg_count - (5+LENGTH asm_conf.avoid_regs)) in
   let p =
     MAP (λ(name_num,arg_count,prog).
@@ -322,12 +322,12 @@ val compile_oracle = store_thm("compile_oracle",``
   fs[next_n_oracle_def]>>
   rveq>>fs[]>>
   match_mp_tac LIST_EQ>>
-  qmatch_goalsub_abbrev_tac`data_to_word$stubs _ ++ p2`
-  \\ qmatch_goalsub_abbrev_tac`MAP f (data_to_word$stubs _)`
+  qmatch_goalsub_abbrev_tac`data_to_word$stubs _ _ ++ p2`
+  \\ qmatch_goalsub_abbrev_tac`MAP f (data_to_word$stubs _ _)`
   \\ REWRITE_TAC[GSYM MAP_APPEND]
   \\ qpat_abbrev_tac`pp = _ ++ p2`
   \\ simp[MAP_MAP_o]
-  \\ qpat_abbrev_tac`len = _ + LENGTH (data_to_word$stubs _)`
+  \\ qpat_abbrev_tac`len = _ + LENGTH (data_to_word$stubs _ _)`
   \\ `len = LENGTH pp` by simp[Abbr`pp`,Abbr`p2`]
   \\ qunabbrev_tac`len` \\ fs[] >>
   rw[]>>fs[EL_MAP,EL_ZIP,full_compile_single_def,compile_single_def,Abbr`f`]>>
