compiler/eval/compilerComputeLib.sml
@@ -385,6 +385,7 @@ val add_compiler_compset = computeLib.extend_compset
     ,data_to_wordTheory.FromList1_code_def
     ,data_to_wordTheory.RefArray_code_def
     ,data_to_wordTheory.Replicate_code_def
+    ,data_to_wordTheory.get_names_def
     ,data_to_wordTheory.assign_def
     ,data_to_wordTheory.comp_def
     ,data_to_wordTheory.compile_part_def
